\p
\begin{enumerate}
\item
$$a_{n+1} - a_n = 3^n$$
$$\Rightarrow a_{n+1} = a_0 + \frac{1}{2}(3^{n+1} - 1) \Rightarrow$$
$$a_n = \frac{1}{2}(3^n + 1)$$
\item
$$a_{n+2} - 2a_{n+1} + a_n = 2^n$$
معادله‌ی فوق را در
$x^{n+2}$
ضرب می‌کنیم:
$$a_{n+2}x^{n+2} - 2a_{n+1}x^{n+2} + a_nx^{n+2} = 2^nx^{n+2}$$
فرض می‌کنیم:
$$f(x) = \sum_{n=0}^{\infty}a_nx^n$$
پس:
$$(f(x) - a_0 - a_1x) - 2x(f(x) - a_0) + x^2f(x) = \sum_{n=0}^{\infty}2^nx^{n+2}$$
$$f(x)(1-2x+x^2)-1-2x+2x = x^2(\frac{1}{1-2x})\Rightarrow f(x) = \frac{1}{1-2x} \Rightarrow a_n = 2^n$$
\end{enumerate}