\p
\begin{enumerate}
\item
$$r^2 - 3r - 4 = 0$$
$$r = -1, 4$$
$$a_n = A(-1)^n + B(4)^n$$
$$1 = A + B$$
$$1 = A + 4B$$
$$B = \frac{2}{5}$$
$$A = \frac{3}{5}$$
$$a_n - \frac{3}{5}(-1)^n + \frac{2}{5}4^n$$
\item
$$r^2 = 1 \Rightarrow r = 1, -1$$
$$a_n = A(-1)^n + B(1)^n$$
$$1 = A + B$$
$$1 = -A + B$$
$$B = 1$$
$$A = 0$$
$$a_n = 1$$
\item
$$r^2 - 2r = 0$$
$$r = 0, 2$$
$$a_n = A2^n$$
$$An^2 + Bn + C = 2A(n-1)^2 + 2B(n-1) + 2C + 2n^2 =$$
$$ n^2(2A + 2) + n(-4A+2B) + 2A - 2B + 2C$$
$$A + 2 = A \Rightarrow A = -2$$
$$4A + 2B = B \Rightarrow B = -8$$
$$2A - 2B + 2C = C \Rightarrow C = 2B - 2A = -16 + 4 = -12$$
$$a_n = A2^n - 2n^2 - 8n - 12$$
$$a_0 = 3 = A - 12 \Rightarrow A = 15$$
$$a_n = 15(2)^n - 2n^2 - 8n - 12$$
\item
بزودی نوشته خواهد شد.
\item
بزودی نوشته خواهد شد.
\end{enumerate}

