\p
\begin{enumerate}
\item
$$a_n + a_{n-1} - 6a_{n-2} = 0$$
معادله‌ی مشخصه:
$$r^2 + r - 6 = 0 \Rightarrow r = 2, -3$$
چون هر دو ریشه حقیقی‌اند، پس هر دوی
$a_n = 2^n$
و
$b_n = (-3)^n$
پاسخ هستند. پس:
$$a_n = c_12^n + c_2(-3)^n$$
$$a_0 = 1 \Rightarrow c_1 + c_2 = 1$$
$$a_1 = 2 \Rightarrow 2c_1 + 3c_2 = 2$$
$$c_2 = 0$$
$$c_1 = 1$$
$$a_n = 2^n$$
\item
$$a_{n+2} = 4a_{n+1} - 4a_n$$
معادله‌ی مشخصه:
$$r^2 - 4r + 4 = 0 \Rightarrow r = 2$$
جواب‌ها
$a_n = c_12^n$
و
$b_n = c_2n2^n$
هستند. پس:
$$a_n = c_12^n + c_2n2^n$$
$$a_0 = 1 \Rightarrow c_1 = 1$$
$$a_1 = 3 \Rightarrow 2c_1 + 2c_2 = 3 \Rightarrow c_2 = \frac{1}{2}$$
$$a_n = 2^n + \frac{1}{2}n2^n$$
$$a_n = 2^n + n2^{n-1}$$
\end{enumerate}